finished interp_instantiate proof and regenerated old interpreter for interactive mode

src/shim.ml
@@ -1,131 +1,130 @@
 
 module type Host = sig
-    include Extract.Executable_Host
-    val show_host_function : host_function -> string
-  end
+  include Extract.Executable_Host
+  val show_host_function : host_function -> string
+end
 
 module DummyHost = struct
-    include Extract.DummyHost
-    let show_host_function _ = assert false
-  end
+  include Extract.DummyHost
+  let show_host_function _ = assert false
+end
 
 module type InterpreterType = sig
 
-    module Host : Host
-    include module type of Host
+  module Host : Host
+  include module type of Host
 
-    val ( >>= ) : 'a host_event -> ('a -> 'b host_event) -> 'b host_event
-    val ( let* ) : 'a host_event -> ('a -> 'b host_event) -> 'b host_event
-    val ( let+ ) : 'a host_event -> ('a -> 'b) -> 'b host_event
-    val ( and+ ) : 'a host_event -> 'b host_event -> ('a * 'b) host_event
-    val pure : 'a -> 'a host_event
+  val ( >>= ) : 'a host_event -> ('a -> 'b host_event) -> 'b host_event
+  val ( let* ) : 'a host_event -> ('a -> 'b host_event) -> 'b host_event
+  val ( let+ ) : 'a host_event -> ('a -> 'b) -> 'b host_event
+  val ( and+ ) : 'a host_event -> 'b host_event -> ('a * 'b) host_event
+  val pure : 'a -> 'a host_event
 
-    type store_record = Extract.EmptyHost.store_record
-    type config_tuple = Extract.config_tuple
-    type res_tuple = Extract.res_tuple
-    type administrative_instruction = Extract.administrative_instruction
+  type store_record = Extract.EmptyHost.store_record
+  type config_tuple = Extract.config_tuple
+  type res_tuple = Extract.res_tuple
+  type administrative_instruction = Extract.administrative_instruction
 
-    val run_v :
-      Extract.nat ->
-      Obj.t * Obj.t Extract.store_record * Extract.frame * administrative_instruction list ->
-      (Obj.t * Obj.t Extract.store_record) * Extract.res
+  val run_v :
+    Extract.nat ->
+    Obj.t * Obj.t Extract.store_record * Extract.frame * administrative_instruction list ->
+    (Obj.t * Obj.t Extract.store_record) * Extract.res
 
-    val run_step_compat :
-      config_tuple -> Extract.res_tuple
+  val run_step_compat :
+    config_tuple -> Extract.res_tuple
 
-    val is_const_list : administrative_instruction list -> Extract.value0 list option
+  val is_const_list : administrative_instruction list -> Extract.value0 list option
 
-    val lookup_exported_function :
-      (* string -> ((store_record * Extract.instance) * Extract.module_export list) -> *)
-      (* config_tuple option *)
-      (* XXX where does "Dune__exe__Extract" come from? should it be exposed? *)
-      string ->
-      (((Extract.Equality.sort * Extract.EmptyHost.store_record) * Extract.instance) * Extract.module_export list) ->
-      (((Extract.Equality.sort * Extract.EmptyHost.store_record) * Extract.frame) * Extract.administrative_instruction list) option
+  val lookup_exported_function :
+    (* string -> ((store_record * Extract.instance) * Extract.module_export list) -> *)
+    (* config_tuple option *)
+    (* XXX where does "Dune__exe__Extract" come from? should it be exposed? *)
+    string ->
+    (((Extract.Equality.sort * Extract.EmptyHost.store_record) * Extract.instance) * Extract.module_export list) ->
+    (((Extract.Equality.sort * Extract.EmptyHost.store_record) * Extract.frame) * Extract.administrative_instruction list) option
 
-    val interp_instantiate_wrapper :
-      (* Extract.module0 -> *)
-      (* (((store_record * Extract.instance) * Extract.module_export list) * int option) option *)
-      Extract.module0 ->
-      ((((Extract.Equality.sort * Extract.EmptyHost.store_record) * Extract.instance) * Extract.module_export list) * Extract.nat option) option
+  val interp_instantiate_wrapper :
+    (* Extract.module0 -> *)
+    (* (((store_record * Extract.instance) * Extract.module_export list) * int option) option *)
+    Extract.module0 ->
+    ((((Extract.Equality.sort * Extract.EmptyHost.store_record) * Extract.instance) * Extract.module_export list) * Extract.nat option) option
 
-    val run_parse_module : string -> Extract.module0 option
+  val run_parse_module : string -> Extract.module0 option
 
-    val pp_values : Extract.value0 list -> string
-    val pp_store : int -> Dune__exe__Extract.EmptyHost.store_record -> string
-    val pp_res_tuple_except_store :
-      ((Extract.EmptyHost.store_record * Extract.frame) * Extract.res_step) -> string
-    val pp_config_tuple_except_store :
-      ((Extract.EmptyHost.store_record * Extract.frame) * Extract.administrative_instruction list) ->
-      string
-    val pp_es : Extract.administrative_instruction list -> string
+  val pp_values : Extract.value0 list -> string
+  val pp_store : int -> Dune__exe__Extract.EmptyHost.store_record -> string
+  val pp_res_tuple_except_store :
+    ((Extract.EmptyHost.store_record * Extract.frame) * Extract.res_step) -> string
+  val pp_config_tuple_except_store :
+    ((Extract.EmptyHost.store_record * Extract.frame) * Extract.administrative_instruction list) ->
+    string
+  val pp_es : Extract.administrative_instruction list -> string
 
-  end
+end
 
 module Interpreter =
-  functor (EH : Host) -> struct
+functor (EH : Host) -> struct
 
-    module Host = EH
-    include Host
+  module Host = EH
+  include Host
 
-    let ( >>= ) = host_bind
+  let ( >>= ) = host_bind
 
-    let ( let* ) = host_bind
+  let ( let* ) = host_bind
 
-    let pure = host_ret
+  let pure = host_ret
 
-    let ( let+ ) a f =
-      let* a = a in
-      pure (f a)
+  let ( let+ ) a f =
+    let* a = a in
+    pure (f a)
 
-    let ( and+ ) a b =
-      let* a = a in
-      let* b = b in
-      pure (a, b)
+  let ( and+ ) a b =
+    let* a = a in
+    let* b = b in
+    pure (a, b)
 
-    (* We are based on the functional version of the interpreter for now *)
-    module Interpreter = Extract.Interpreter_func_extract
-    module Instantiation = Extract.Instantiation_func_extract
-    module PP = Extract.PP
+  (* We are based on the functional version of the interpreter for now *)
+  module Interpreter = Extract.Interpreter_func_extract
+  module Instantiation = Extract.Instantiation_func_extract
+  module PP = Extract.PP
 
-    type store_record = Extract.EmptyHost.store_record
-    type config_tuple = Extract.config_tuple
-    type res_tuple = Extract.res_tuple
-    type administrative_instruction = Extract.administrative_instruction
+  type store_record = Extract.EmptyHost.store_record
+  type config_tuple = Extract.config_tuple
+  type res_tuple = Extract.res_tuple
+  type administrative_instruction = Extract.administrative_instruction
 
-    let run_v i cfg =
-      let (hs, s, f, es) = cfg in
-      Interpreter.run_v hs s f es i
+  let run_v i cfg =
+    let (hs, s, f, es) = cfg in
+    Interpreter.run_v hs s f es i
 
-    let run_step_compat cfg =
-      Interpreter.run_step_compat cfg
+  let run_step_compat cfg =
+    Interpreter.run_step_compat cfg
 
-    let is_const_list = Interpreter.is_const_list
+  let is_const_list = Interpreter.is_const_list
 
-    let lookup_exported_function name =
-      Instantiation.lookup_exported_function (Utils.explode name)
+  let lookup_exported_function name =
+    Instantiation.lookup_exported_function (Utils.explode name)
 
-    let interp_instantiate_wrapper m =
-      Instantiation.interp_instantiate_wrapper m
+  let interp_instantiate_wrapper m =
+    Instantiation.interp_instantiate_wrapper m
 (*
-    let show_host_function_char_list h = Utils.explode (show_host_function h)
+  let show_host_function_char_list h = Utils.explode (show_host_function h)
 *)
-    let run_parse_module m = Extract.run_parse_module (Utils.explode m)
+  let run_parse_module m = Extract.run_parse_module (Utils.explode m)
 
-    let pp_values l =
-      Utils.implode (PP.pp_values l)
+  let pp_values l =
+    Utils.implode (PP.pp_values l)
 
-    let pp_store i st =
-      Utils.implode (PP.pp_store (Convert.to_nat i) st)
+  let pp_store i st =
+    Utils.implode (PP.pp_store (Convert.to_nat i) st)
 
-    let pp_res_tuple_except_store r =
-      Utils.implode (PP.pp_res_tuple_except_store r)
+  let pp_res_tuple_except_store r =
+    Utils.implode (PP.pp_res_tuple_except_store r)
 
-    let pp_config_tuple_except_store cfg =
-      Utils.implode (PP.pp_config_tuple_except_store cfg)
+  let pp_config_tuple_except_store cfg =
+    Utils.implode (PP.pp_config_tuple_except_store cfg)
 
-    let pp_es es =
-      Utils.implode (PP.pp_administrative_instructions O es)
+  let pp_es es =
+    Utils.implode (PP.pp_administrative_instructions O es)
 
-  end
-
+end
