src/shim.mli
@@ -2,95 +2,94 @@
 
 module type Host = sig
 
-    (** The type of host functions. *)
-    type host_function
+  (** The type of host functions. *)
+  type host_function
 
-    (** Equality of host functions. *)
-    val host_function_eq_dec : host_function -> host_function -> bool
+  (** Equality of host functions. *)
+  val host_function_eq_dec : host_function -> host_function -> bool
 
-    (** The monad of host events. *)
-    type 'a host_event
-    val host_ret : 'a -> 'a host_event
-    val host_bind : 'a host_event -> ('a -> 'b host_event) -> 'b host_event
+  (** The monad of host events. *)
+  type 'a host_event
+  val host_ret : 'a -> 'a host_event
+  val host_bind : 'a host_event -> ('a -> 'b host_event) -> 'b host_event
 
-    (** Application of a host function in the host monad. *)
-    val host_apply :
-      host_function Extract.store_record -> Extract.function_type -> host_function -> Extract.value0 list ->
-      (host_function Extract.store_record * Extract.result) option host_event
+  (** Application of a host function in the host monad. *)
+  val host_apply :
+    host_function Extract.store_record -> Extract.function_type -> host_function -> Extract.value0 list ->
+    (host_function Extract.store_record * Extract.result) option host_event
 
-    (** Printing a host function. *)
-    val show_host_function : host_function -> string
-  end
+  (** Printing a host function. *)
+  val show_host_function : host_function -> string
+end
 
 module DummyHost : Host
 
 module type InterpreterType = sig
 
-    module Host : Host
-    include module type of Host
+  module Host : Host
+  include module type of Host
 
-    (** The usual monadic notations. *)
-    val ( >>= ) : 'a host_event -> ('a -> 'b host_event) -> 'b host_event
-    val ( let* ) : 'a host_event -> ('a -> 'b host_event) -> 'b host_event
-    val ( let+ ) : 'a host_event -> ('a -> 'b) -> 'b host_event
-    val ( and+ ) : 'a host_event -> 'b host_event -> ('a * 'b) host_event
-    val pure : 'a -> 'a host_event
+  (** The usual monadic notations. *)
+  val ( >>= ) : 'a host_event -> ('a -> 'b host_event) -> 'b host_event
+  val ( let* ) : 'a host_event -> ('a -> 'b host_event) -> 'b host_event
+  val ( let+ ) : 'a host_event -> ('a -> 'b) -> 'b host_event
+  val ( and+ ) : 'a host_event -> 'b host_event -> ('a * 'b) host_event
+  val pure : 'a -> 'a host_event
 
-    type store_record = Extract.EmptyHost.store_record
-    type config_tuple = Extract.config_tuple
-    type res_tuple = Extract.res_tuple
-    type administrative_instruction = Extract.administrative_instruction
+  type store_record = Extract.EmptyHost.store_record
+  type config_tuple = Extract.config_tuple
+  type res_tuple = Extract.res_tuple
+  type administrative_instruction = Extract.administrative_instruction
 
-    (** Run the interpreter until reaching a result. *)
-    (* val run_v : *)
-    (*   Extract.instance -> config_tuple -> *)
-    (*   (store_record * Extract.res) host_event *)
+  (** Run the interpreter until reaching a result. *)
+  (* val run_v : *)
+  (*   Extract.instance -> config_tuple -> *)
+  (*   (store_record * Extract.res) host_event *)
 
-    val run_v :
-      Extract.nat ->
-      Obj.t * Obj.t Extract.store_record * Extract.frame * administrative_instruction list ->
-      (Obj.t * Obj.t Extract.store_record) * Extract.res
+  val run_v :
+    Extract.nat ->
+    Obj.t * Obj.t Extract.store_record * Extract.frame * administrative_instruction list ->
+    (Obj.t * Obj.t Extract.store_record) * Extract.res
 
-    (** Run one step of the interpreter. *)
-    val run_step_compat :
-      config_tuple -> Extract.res_tuple
+  (** Run one step of the interpreter. *)
+  val run_step_compat :
+    config_tuple -> Extract.res_tuple
 
-    (** State whether a list of administrative instructions is actually just a list of values. *)
-    val is_const_list : administrative_instruction list -> Extract.value0 list option
+  (** State whether a list of administrative instructions is actually just a list of values. *)
+  val is_const_list : administrative_instruction list -> Extract.value0 list option
 
-    (** Look-up a specific extracted function of the instantiation. *)
-    val lookup_exported_function :
-      (* string -> (store_record * Extract.instance) * Extract.module_export list -> *)
-      (* config_tuple option *)
-      string ->
-      (((Extract.Equality.sort * Extract.EmptyHost.store_record) * Extract.instance) * Extract.module_export list) ->
-      (((Extract.Equality.sort * Extract.EmptyHost.store_record) * Extract.frame) * Extract.administrative_instruction list) option
+  (** Look-up a specific extracted function of the instantiation. *)
+  val lookup_exported_function :
+    (* string -> (store_record * Extract.instance) * Extract.module_export list -> *)
+    (* config_tuple option *)
+    string ->
+    (((Extract.Equality.sort * Extract.EmptyHost.store_record) * Extract.instance) * Extract.module_export list) ->
+    (((Extract.Equality.sort * Extract.EmptyHost.store_record) * Extract.frame) * Extract.administrative_instruction list) option
 
-    (** Perform the instantiation of a module. *)
-    val interp_instantiate_wrapper :
-      Extract.module0 ->
-      ((((Extract.Equality.sort * Extract.EmptyHost.store_record) * Extract.instance) * Extract.module_export list) * Extract.nat option) option
+  (** Perform the instantiation of a module. *)
+  val interp_instantiate_wrapper :
+    Extract.module0 ->
+    ((((Extract.Equality.sort * Extract.EmptyHost.store_record) * Extract.instance) * Extract.module_export list) * Extract.nat option) option
 
-    (** Parsing. *)
+  (** Parsing. *)
 
-    val run_parse_module : string -> Extract.module0 option
+  val run_parse_module : string -> Extract.module0 option
 
-    (** Pretty-printing. *)
+  (** Pretty-printing. *)
 
-    val pp_values : Extract.value0 list -> string
-    val pp_store : int (** The indentation level *) -> store_record -> string
-    val pp_res_tuple_except_store :
-      ((Extract.EmptyHost.store_record * Extract.frame) * Extract.res_step) -> string
-    val pp_config_tuple_except_store :
-      ((Extract.EmptyHost.store_record * Extract.frame) * Extract.administrative_instruction list) ->
-      string
-    val pp_es : Extract.administrative_instruction list -> string
+  val pp_values : Extract.value0 list -> string
+  val pp_store : int (** The indentation level *) -> store_record -> string
+  val pp_res_tuple_except_store :
+    ((Extract.EmptyHost.store_record * Extract.frame) * Extract.res_step) -> string
+  val pp_config_tuple_except_store :
+    ((Extract.EmptyHost.store_record * Extract.frame) * Extract.administrative_instruction list) ->
+    string
+  val pp_es : Extract.administrative_instruction list -> string
 
 
-  end
+end
 
 module Interpreter : functor (EH : Host) ->
-  InterpreterType
-    with module Host = EH
-    and type 'a host_event = 'a EH.host_event
-
+InterpreterType
+  with module Host = EH
+  and type 'a host_event = 'a EH.host_event
